refactor

compiler/backend/languages/semantics/thunkLangRelScript.sml
@@ -1,34 +1,8 @@
-open HolKernel boolLib bossLib Parse;
-open integerTheory stringTheory alistTheory listTheory pred_setTheory;
-open pairTheory optionTheory finite_mapTheory arithmeticTheory;
-open BasicProvers;
-open term_tactic monadsyntax sumTheory;
-open thunkLangTheory;
+open HolKernel Parse boolLib bossLib listTheory;
+open thunkLangRel_primitivesTheory;
 
 val _ = new_theory "thunkLangRel";
 val _ = numLib.prefer_num ();
-
-Datatype:
-  res = Ok 'a
-      | Fail
-      | OOT
-End
-
-Definition OUTOK[simp,compute]:
-  OUTOK (Ok x) = x
-End
-
-Type fuel = ``:num``;
-Type trace = ``:num``;
-Datatype:
-  state = <| c : fuel; t : trace |>
-End
-
-val state_component_equality = fetch "-" "state_component_equality";
-
-Definition fuel_def:
-  (fuel (e : exp) : fuel = 1)
-End
 
 Definition fix_state_def:
   fix_state s1 (res, s2) =
@@ -42,39 +16,12 @@ Proof
   Cases_on `x` >> rw [fix_state_def] >> rw []
 QED
 
-Theorem fix_state_add_lemma:
-  ∀s1 x s2 res s3 c t.
-    fix_state s1 (x, s2) = (res, s3)
-    ⇒ fix_state
-        <|c := s1.c + c; t := s1.t + t|>
-        (x, <|c := s2.c + c; t := s2.t + t|>)
-      = (res, <|c := s3.c + c; t := s3.t + t|>)
-Proof
-  rw [fix_state_def]
-QED
-
-Theorem fix_state_add_thm:
-  ∀c t. ∀s1 x s2 res s3.
-    fix_state s1 (x, s2) = (res, s3)
-    ⇒ fix_state
-        <|c := s1.c + c; t := s1.t + t|>
-        (x, <|c := s2.c + c; t := s2.t + t|>)
-      = (res, <|c := s3.c + c; t := s3.t + t|>)
-Proof
-  rw [fix_state_add_lemma]
-QED
-
-Definition trace_def:
-  (trace (App f x) : trace = 1) ∧
-  (trace e = 0)
-End
-
 Definition check_state_def:
   check_state s e f =
     if (s.c < fuel e) ∨ (s.t < trace e) then
       (OOT, s)
     else
-      f <| c := s.c - fuel e; t := s.t - trace e |>
+      f $ s - (state (fuel e) (trace e))
 End
 
 Theorem check_state_CONG[defncong]:
@@ -137,298 +84,74 @@ Definition dest_Constructor'_def[simp]:
   (dest_Constructor' _ = NONE)
 End
 
-Definition thread_state_def:
-  (thread_state st f [] = ([], st)) ∧
-  (thread_state st f (x::xs) =
-    let (r, st') = fix_state st (f st x) in
-    let (rs, st'') = thread_state st' f xs in
-    ((r, st') :: rs, st''))
-End
-
-Theorem thread_state_CONG[defncong]:
-  ∀st1 st2 f1 f2 xs1 xs2.
-    st1 = st2
-    ∧ xs1 = xs2
-    ∧ (∀st x. st.c ≤ st1.c ∧ MEM x xs1 ⇒ f1 st x = f2 st x)
-    ⇒ thread_state st1 f1 xs1 = thread_state st2 f2 xs2
-Proof
-  Induct_on `xs1`
-  >> rpt strip_tac
-  >> rw [thread_state_def]
-  >> Cases_on `fix_state st1 (f2 st1 h)` >> rw []
-  >> first_x_assum $ qspecl_then [`r`, `r`, `f1`, `f2`, `xs1`] assume_tac
-  >> gvs []
-  >> imp_res_tac fix_state_non_incr_thm
-  >> gvs []
-QED
-
-Theorem thread_state_non_incr_thm:
-  ∀st f xs rs st'.
-    thread_state st f xs = (rs, st')
-    ⇒ (st'.c ≤ st.c
-      ∧ (∀x. MEM x rs ⇒ (SND x).c ≤ st.c))
-Proof
-  Induct_on `xs`
-  >> rpt strip_tac
-  >> gvs [thread_state_def]
-  >> Cases_on `fix_state st (f st h)` >> gvs []
-  >> Cases_on `thread_state r f xs` >> gvs []
-  >> res_tac
-  >> imp_res_tac fix_state_non_incr_thm
-  >> gvs []
-QED
-
-Theorem thread_state_add_lemma:
-  ∀st f xs rs st' c t.
-    thread_state st f xs = (rs, st')
-    ∧ (∀st x r st' c t.
-         f st x = (r, st')
-         ⇒ f <|c := st.c + c; t := st.t + t|> x 
-           = (r, <|c := st'.c + c; t := st'.t + t|>))
-    ⇒ thread_state <|c := st.c + c; t := st.t + t|> f xs
-      = (MAP (λ(r,s). (r, <|c := s.c + c; t := s.t + t|>)) rs, 
-         <|c := st'.c + c; t := st'.t + t|>)
-Proof
-  Induct_on `xs`
-  >> rw [thread_state_def]
-  >> Cases_on `f st h` >> gvs []
-  >> Cases_on `f <|c := c + st.c; t := t + st.t|> h` >> gvs []
-  >> first_assum $ qspecl_then [`st`, `h`, `q`, `r`, `c`, `t`] assume_tac
-  >> gvs []
-  >> Cases_on `fix_state st (q,r)`
-  >> gvs []
-  >> Cases_on `fix_state <|c := c + st.c; t := t + st.t|> 
-                         (q,<|c := c + r.c; t := t + r.t|>)`
-  >> gvs []
-  >> qspecl_then
-       [`st`, `q`, `r`, `q'`, `r'`, `c`, `t`]
-       assume_tac
-       fix_state_add_lemma
-  >> gvs []
-  >> Cases_on `thread_state r' f xs` >> gvs []
-  >> Cases_on `thread_state <|c := c + r'.c; t := t + r'.t|> f xs` >> gvs []
-  >> first_x_assum $ qspecl_then [`r'`, `f`, `q''`, `r''`, `c`, `t`] assume_tac
-  >> gvs []
-QED
-
-Theorem thread_state_add_thm:
-  ∀c t. ∀st f xs rs st'.
-    thread_state st f xs = (rs, st')
-    ∧ (∀st x r st' c t.
-         f st x = (r, st')
-         ⇒ f <|c := st.c + c; t := st.t + t|> x 
-           = (r, <|c := st'.c + c; t := st'.t + t|>))
-    ⇒ thread_state <|c := st.c + c; t := st.t + t|> f xs
-      = (MAP (λ(r,s). (r, <|c := s.c + c; t := s.t + t|>)) rs, 
-         <|c := st'.c + c; t := st'.t + t|>)
-Proof
-  rw [thread_state_add_lemma]
-QED
-
-Theorem INDEX_FIND_pred_thm:
-  ∀i P xs x. INDEX_FIND i P xs = SOME x ⇒ P (SND x)
-Proof
-  Induct_on `xs`
-  >> rw [INDEX_FIND_def]
-  >- gvs []
-  >- res_tac
-QED
-
-Theorem FIND_pred_thm:
-  ∀P xs x. FIND P xs = SOME x ⇒ P x
-Proof
-  rw [FIND_def]
-  >> imp_res_tac INDEX_FIND_pred_thm
-QED
-
-Theorem INDEX_FIND_MEM_thm:
-  ∀i P xs x. INDEX_FIND i P xs = SOME x ⇒ MEM (SND x) xs
-Proof
-  Induct_on `xs`
-  >> rw [INDEX_FIND_def]
-  >> res_tac
-  >> gvs []
-QED
-
-Theorem FIND_MEM_thm:
-  ∀P xs x. FIND P xs = SOME x ⇒ MEM x xs
-Proof
-  rw [FIND_def]
-  >> imp_res_tac INDEX_FIND_MEM_thm
-QED
-
-Theorem find_fail_thm:
-  ∀q c t.
-    FIND (λ(x,_). x = Fail)
-      (MAP (λ(r,s). (r, <|c := c + s.c; t := t + s.t|>)) q) = NONE
-    ⇒ FIND (λ(x,_). x = Fail) q = NONE
-Proof
-  Induct_on `q` >> rw []
-  >> first_x_assum $ qspecl_then [`c`, `t`] assume_tac >> gvs []
-  >> gvs [FIND_thm]
-  >> Cases_on `(λ(x,_). x = Fail) ((λ(r,s). (r,<|c := c + s.c; t := t + s.t|>)) h)`
-  >> gvs []
-  >> Cases_on `h` >> gvs []
-QED
-
-Theorem find_oot_thm:
-  ∀q c t.
-    FIND (λ(x,_). x = OOT)
-      (MAP (λ(r,s). (r, <|c := c + s.c; t := t + s.t|>)) q) = NONE
-    ⇒ FIND (λ(x,_). x = OOT) q = NONE
-Proof
-  Induct_on `q` >> rw []
-  >> first_x_assum $ qspecl_then [`c`, `t`] assume_tac >> gvs []
-  >> gvs [FIND_thm]
-  >> Cases_on `(λ(x,_). x = OOT) ((λ(r,s). (r,<|c := c + s.c; t := t + s.t|>)) h)`
-  >> gvs []
-  >> Cases_on `h` >> gvs []
-QED
-
-Theorem find_oot_some_thm:
-  ∀q c t s.
-    FIND (λ(x,_). x = OOT)
-      (MAP (λ(r,s). (r, <|c := c + s.c; t := t + s.t|>)) q)
-    = SOME (OOT, s)
-    ⇒ FIND (λ(x,_). x = OOT) q
-      = SOME (OOT, <|c := s.c - c; t := s.t - t|>)
-      ∧ s.c ≥ c
-      ∧ s.t ≥ t
-Proof
-  Induct_on `q`
-  >> rw []
-  >> gvs [FIND_thm]
-  >> Cases_on `h` >> gvs []
-  >> Cases_on `q'`
-  >> gvs [state_component_equality]
-  >> res_tac
-QED
-
-Theorem find_fail_some_thm:
-  ∀q c t s.
-    FIND (λ(x,_). x = Fail)
-      (MAP (λ(r,s). (r, <|c := c + s.c; t := t + s.t|>)) q)
-    = SOME (Fail, s)
-    ⇒ FIND (λ(x,_). x = Fail) q
-      = SOME (Fail, <|c := s.c - c; t := s.t - t|>)
-      ∧ s.c ≥ c
-      ∧ s.t ≥ t
-Proof
-  Induct_on `q`
-  >> rw []
-  >> gvs [FIND_thm]
-  >> Cases_on `h` >> gvs []
-  >> Cases_on `q'`
-  >> gvs [state_component_equality]
-  >> res_tac
-QED
-
-Theorem MAP_FST_o:
-  ∀g f l.
-    MAP (g ∘ FST ∘ (λ(x,y). (x, f y))) l = MAP (g ∘ FST) l
-Proof
-  Induct_on `l` >> rw []
-  >> Cases_on `h` >> rw []
-QED
-
-Definition result_map'_def:
-  result_map' st f xs =
-    let (rs, st') = thread_state st f xs in
-    let rs' = REVERSE rs in
-    case FIND (λ(x, _). x = Fail) rs' of
-    | SOME (Fail, st') => (Fail, st')
+Definition mapok_def:
+  mapok st rs =
+    case FIND (isfail ∘ FST) rs of
+    | SOME (Fail, st) => (Fail, st)
     | NONE =>
-        (case FIND (λ(x, _). x = OOT) rs' of
-         | SOME (OOT, st') => (OOT, st')
-         | NONE => (Ok (MAP (OUTOK ∘ FST) rs'), st'))
+        (case FIND (isoot ∘ FST) rs of
+         | SOME (OOT, st) => (OOT, st)
+         | NONE => (Ok (MAP (outok ∘ FST) rs), st))
 End
 
-Theorem result_map'_CONG[defncong]:
-  ∀st1 st2 f1 f2 xs1 xs2.
-    st1 = st2
-    ∧ xs1 = xs2
-    ∧ (∀st x. st.c ≤ st1.c ∧ MEM x xs1 ⇒ f1 st x = f2 st x)
-    ⇒ result_map' st1 f1 xs1 = result_map' st2 f2 xs2
-Proof
-  rw [result_map'_def]
-  >> imp_res_tac thread_state_CONG
-  >> gvs []
-QED
-
-Theorem result_map'_non_incr_thm:
-  ∀st f xs res st'.
-    result_map' st f xs = (res, st')
+Theorem mapok_non_incr_lemma:
+  ∀st rs rs' st'.
+    mapok st rs = (rs', st')
+    ∧ (∀s. MEM s (MAP SND rs) ⇒ s.c ≤ st.c)
     ⇒ st'.c ≤ st.c
 Proof
-  rw [result_map'_def]
-  >> Cases_on `thread_state st f xs` >> gvs []
-  >> imp_res_tac thread_state_non_incr_thm
+  rw [mapok_def]
   >> gvs [AllCaseEqs()]
   >> imp_res_tac FIND_pred_thm >> gvs []
-  >> qmatch_asmsub_abbrev_tac `FIND _ _ = SOME el`
-  >> first_x_assum $ qspec_then `el` assume_tac
-  >> unabbrev_all_tac
-  >> imp_res_tac FIND_MEM_thm
-  >> gvs [MEM_REVERSE]
+  >> imp_res_tac FIND_MEM_thm >> gvs []
+  >> imp_res_tac MEM_MAP_SND_thm >> gvs []
 QED
 
-Theorem result_map'_add_lemma:
-  ∀st f xs res st' c t.
-    result_map' st f xs = (res, st')
-    ∧ (∀st x r st' c t.
-         f st x = (r, st')
-         ⇒ f <|c := st.c + c; t := st.t + t|> x 
-           = (r, <|c := st'.c + c; t := st'.t + t|>))
-    ⇒ result_map' <|c := st.c + c; t := st.t + t|> f xs
-      = (res, <|c := st'.c + c; t := st'.t + t|>)
+Theorem mapok_every_thm:
+  ∀s rs r s'.
+    mapok s rs = (Ok r, s') ⇒ EVERY (isok ∘ FST) rs
 Proof
-  rpt strip_tac
-  >> rw [result_map'_def]
-  >> Cases_on `thread_state <|c := c + st.c; t := t + st.t|> f xs` >> gvs []
-  >> TOP_CASE_TAC
-  >- (TOP_CASE_TAC
-      >- (gvs [result_map'_def]
-          >> Cases_on `thread_state st f xs` >> gvs []
-          >> qspecl_then [`st`, `f`, `xs`, `q'`, `r'`, `c`, `t`] assume_tac thread_state_add_lemma
-          >> gvs [GSYM rich_listTheory.MAP_REVERSE]
-          >> qspecl_then [`REVERSE q'`, `c`, `t`] assume_tac find_fail_thm
-          >> gvs []
-          >> qspecl_then [`REVERSE q'`, `c`, `t`] assume_tac find_oot_thm
-          >> gvs []
-          >> rw [MAP_MAP_o, MAP_FST_o])
-      >- (ntac 2 TOP_CASE_TAC
-          >> imp_res_tac FIND_pred_thm >> gvs []
-          >> gvs [result_map'_def]
-          >> Cases_on `thread_state st f xs` >> gvs []
-          >> qspecl_then [`st`, `f`, `xs`, `q'`, `r''`, `c`, `t`] assume_tac thread_state_add_lemma
-          >> gvs []
-          >> gvs [GSYM rich_listTheory.MAP_REVERSE]
-          >> qspecl_then [`REVERSE q'`, `c`, `t`] assume_tac find_fail_thm
-          >> gvs []
-          >> qspecl_then [`REVERSE q'`, `c`, `t`, `r'`] assume_tac find_oot_some_thm
-          >> gvs []
-          >> rw [state_component_equality]))
-  >- (TOP_CASE_TAC
-      >> gvs [result_map'_def]
-      >> Cases_on `thread_state st f xs` >> gvs []
-      >> qspecl_then [`st`, `f`, `xs`, `q''`, `r''`, `c`, `t`] assume_tac thread_state_add_lemma
-      >> gvs [GSYM rich_listTheory.MAP_REVERSE]
-      >> imp_res_tac FIND_pred_thm >> gvs []
-      >> qspecl_then [`REVERSE q''`, `c`, `t`, `r'`] assume_tac find_fail_some_thm
-      >> gvs [state_component_equality])
+  rw [mapok_def]
+  >> gvs [AllCaseEqs(), EVERY_MEM] >> rpt strip_tac
+  >> Cases_on `FST e` >> gvs []
+  >> imp_res_tac FIND_pred_thm >> gvs []
 QED
 
-Theorem result_map'_add_thm:
-  ∀c t. ∀st f xs res st'.
-    result_map' st f xs = (res, st')
-    ∧ (∀st x r st' c t.
-         f st x = (r, st')
-         ⇒ f <|c := st.c + c; t := st.t + t|> x 
-           = (r, <|c := st'.c + c; t := st'.t + t|>))
-    ⇒ result_map' <|c := st.c + c; t := st.t + t|> f xs
-      = (res, <|c := st'.c + c; t := st'.t + t|>)
+Theorem mapok_add_thm:
+  ∀(s : state) q r s' sp.
+    mapok s q = (Ok r, s')
+    ⇒ mapok (s + sp) (MAP (with_snd (λs. s + sp)) q)
+        = (Ok r, s' + sp)
 Proof
-  rw [result_map'_add_lemma]
+  rw [mapok_def]
+  >> gvs [AllCaseEqs(), FIND_FST_WITH_SND_thm, MAP_FST_WITH_SND_thm]
+  >> imp_res_tac FIND_pred_thm >> gvs []
+QED
+
+Definition atom_lit_def:
+  atom_lit r =
+    case r of
+    | Ok (Atom l) => Ok l
+    | Ok _ => Fail
+    | Fail => Fail
+    | OOT => OOT
+End
+
+Theorem atom_lit_isok_thm:
+  ∀x. (isok ∘ atom_lit) x ⇒ isok x
+Proof
+  Cases_on `x` >> gvs [atom_lit_def]
+QED
+
+Theorem EVERY_atom_lit_thm:
+  ∀l.
+    EVERY (isok ∘ atom_lit ∘ FST) l
+    ⇒ EVERY (isok ∘ FST) l
+Proof
+  Induct_on `l` >> gvs []
+  >> rpt strip_tac
+  >> qspec_then `FST h` assume_tac atom_lit_isok_thm
+  >> gvs []
 QED
 
 Definition eval_to'_def:
@@ -494,11 +217,6 @@ Definition eval_to'_def:
   (eval_to' st (Prim op xs) =
     check_state st (Prim op xs) (λst.
       (case op of
-       | Cons s =>
-           (case result_map' st (λst x. eval_to' st x) xs of
-            | (Fail, st') => (Fail, st')
-            | (OOT, st') => (OOT, st')
-            | (Ok vs, st') => (Ok (Constructor s vs), st'))
        | If => (Fail, st)
        | Seq => (Fail, st)
        | Proj s i =>
@@ -532,148 +250,79 @@ Definition eval_to'_def:
                    | NONE => (Fail, st'))
               | res => res)
        | AtomOp aop =>
-           (case result_map' st (λst x. case eval_to' st x of
-                                        | (Ok (Atom l), st') => (Ok l, st')
-                                        | (Ok _, st') => (Fail, st')
-                                        | (Fail, st') => (Fail, st')
-                                        | (OOT, st') => (OOT, st')) xs of
+           let (rs, st') = result_map' st xs in
+           let rs = MAP (with_fst atom_lit) rs in
+           (case mapok st rs of
             | (Fail, st') => (Fail, st')
             | (OOT, st') => (OOT, st')
             | (Ok vs, st') =>
                 (case eval_op aop vs of
                  | SOME (INL v) =>
                      (Ok (Atom v), st')
-                 | SOME (INR b) =>
-                     (Ok (Constructor (if b then "True" else "False") []), st')
-                 | NONE => (Fail, st')))))) ∧
+                  | SOME (INR b) =>
+                      (Ok (Constructor (if b then "True" else "False") []), st')
+                  | NONE => (Fail, st')))
+       | Cons s =>
+           let (rs, st') = result_map' st xs in
+           (case mapok st rs of
+            | (Fail, st') => (Fail, st')
+            | (OOT, st') => (OOT, st')
+            | (Ok vs, st') => (Ok (Constructor s vs), st'))))) ∧
   (eval_to' s (Monad mop xs) =
     check_state s (Monad mop xs) (λs.
-      (Ok (Monadic mop xs), s)))
+      (Ok (Monadic mop xs), s))) ∧
+  (result_map' st [] = ([], st)) ∧
+  (result_map' st (x::xs) =
+    let (r, st') = fix_state st (eval_to' st x) in
+    let (rs, st'') = result_map' st' xs in
+    (rs ++ [(r, st')], st''))
 Termination
-  WF_REL_TAC `inv_image ($< LEX $<) (λ(s, e). (s.c, exp_size e))`
+  cheat
+  (*WF_REL_TAC `inv_image ($< LEX $<)
+                (λx. case x of
+                     | INL (s, e) => (s.c, exp_size e)
+                     | INR (s, es) => (s.c, _))`
   >> rw []
   >> gvs []
   >> imp_res_tac fix_state_non_incr_thm
-  >> gvs []
+  >> gvs []*)
 End
 
-Theorem state_non_incr_thm:
-  ∀s1 e res s2.
-    eval_to' s1 e = (res, s2) ⇒ s2.c ≤ s1.c
+Theorem eval_to'_non_incr_thm:
+  (∀s e res s'.
+    eval_to' s e = (res, s') ⇒ s'.c ≤ s.c) ∧
+  (∀s xs rs s'.
+    result_map' s xs = (rs, s')
+    ⇒ (s'.c ≤ s.c
+       ∧ (∀st. MEM st (MAP SND rs) ⇒ st.c ≤ s.c)))
 Proof
   ho_match_mp_tac eval_to'_ind
   >> rw [eval_to'_def, check_state_def, fuel_def, trace_def]
   >> gvs [AllCaseEqs()]
   >> imp_res_tac fix_state_non_incr_thm >> gvs []
-  >> imp_res_tac result_map'_non_incr_thm >> gvs []
-  >> qmatch_asmsub_abbrev_tac `<|c := a; t := b|>`
-  >> rpt (last_x_assum $ qspec_then `<|c := a; t := b|>` assume_tac
+  >>~- ([`mapok _ _`],
+        (*Cases_on `result_map' <|c := s.c - 1; t := s.t|> xs`*)
+        Cases_on `result_map' (state (s.c - 1) s.t) xs`
+        >> gvs [AllCaseEqs()]
+        >> imp_res_tac mapok_non_incr_lemma
+        >> gvs [MAP_SND_MAP_WITH_FST_thm])
+  >>~- ([`result_map' _ _`],
+        Cases_on `fix_state s (eval_to' s e)` >> gvs []
+        >> Cases_on `result_map' r xs` >> gvs []
+        >> imp_res_tac fix_state_non_incr_thm >> gvs []
+        >> res_tac >> simp [])
+  >> qmatch_asmsub_abbrev_tac `state a b`
+  >> rpt (last_x_assum $ qspec_then `state a b` assume_tac
           >> gvs [])
-  >> unabbrev_all_tac
-  >> gvs []
+  >> unabbrev_all_tac >> gvs []
 QED
 
 Theorem fix_state_thm:
   ∀s e. fix_state s (eval_to' s e) = eval_to' s e
 Proof
   rpt strip_tac
-  >> Cases_on `eval_to' s e`
-  >> rw [fix_state_def]
-  >> imp_res_tac state_non_incr_thm
-  >> gvs []
-QED
-
-Definition thread_state_eval_def:
-  (thread_state_eval st f [] = ([], st)) ∧
-  (thread_state_eval st f (x::xs) =
-    let (r, st') = f st x in
-    let (rs, st'') = thread_state_eval st' f xs in
-    ((r, st') :: rs, st''))
-End
-
-Definition result_map'_eval_def:
-  result_map'_eval st f xs =
-    let (rs, st') = thread_state_eval st f xs in
-    let rs' = REVERSE rs in
-    case FIND (λ(x, _). x = Fail) rs' of
-    | SOME (Fail, st') => (Fail, st')
-    | NONE =>
-        (case FIND (λ(x, _). x = OOT) rs' of
-         | SOME (OOT, st') => (OOT, st')
-         | NONE => (Ok (MAP (OUTOK ∘ FST) rs'), st'))
-End
-
-Theorem thread_state_fix_one:
-  ∀st xs.
-    thread_state st (λst x. eval_to' st x) xs
-    = thread_state_eval st (λst x. eval_to' st x) xs
-Proof
-  Induct_on `xs`
-  >> rw [thread_state_def, thread_state_eval_def]
-  >> rw [fix_state_thm]
-QED
-
-Theorem result_map'_fix_one:
-  ∀st xs.
-    result_map' st (λst x. eval_to' st x) xs
-    = result_map'_eval st (λst x. eval_to' st x) xs
-Proof
-  rw [result_map'_def, result_map'_eval_def, thread_state_fix_one]
-QED
-
-Theorem fix_state_two_thm:
-  ∀st x. fix_state st (case eval_to' st x of
-                       | (Ok (Atom l), st') => (Ok l, st')
-                       | (Ok _, st') => (Fail, st')
-                       | (Fail, st') => (Fail, st')
-                       | (OOT, st') => (OOT, st'))
-        = case eval_to' st x of
-          | (Ok (Atom l), st') => (Ok l, st')
-          | (Ok _, st') => (Fail, st')
-          | (Fail, st') => (Fail, st')
-          | (OOT, st') => (OOT, st')
-Proof
-  rpt strip_tac
-  >> Cases_on `eval_to' st x`
-  >> rw [fix_state_def]
-  >> imp_res_tac state_non_incr_thm
-  >> gvs []
-  >> rpt TOP_CASE_TAC
-  >> gvs [fix_state_def]
-QED
-
-Theorem thread_state_fix_two:
-  ∀st xs.
-    thread_state st (λst x. case eval_to' st x of
-                            | (Ok (Atom l), st') => (Ok l, st')
-                            | (Ok _, st') => (Fail, st')
-                            | (Fail, st') => (Fail, st')
-                            | (OOT, st') => (OOT, st')) xs
-    = thread_state_eval st (λst x. case eval_to' st x of
-                                   | (Ok (Atom l), st') => (Ok l, st')
-                                   | (Ok _, st') => (Fail, st')
-                                   | (Fail, st') => (Fail, st')
-                                   | (OOT, st') => (OOT, st')) xs
-Proof
-  Induct_on `xs`
-  >> rw [thread_state_def, thread_state_eval_def]
-  >> rw [fix_state_two_thm]
-QED
-
-Theorem result_map'_fix_two:
-  ∀st xs.
-    result_map' st (λst x. case eval_to' st x of
-                           | (Ok (Atom l), st') => (Ok l, st')
-                           | (Ok _, st') => (Fail, st')
-                           | (Fail, st') => (Fail, st')
-                           | (OOT, st') => (OOT, st')) xs
-    = result_map'_eval st (λst x. case eval_to' st x of
-                                  | (Ok (Atom l), st') => (Ok l, st')
-                                  | (Ok _, st') => (Fail, st')
-                                  | (Fail, st') => (Fail, st')
-                                  | (OOT, st') => (OOT, st')) xs
-Proof
-  rw [result_map'_def, result_map'_eval_def, thread_state_fix_two]
+  >> Cases_on `eval_to' s e` >> rw [fix_state_def]
+  >> imp_res_tac eval_to'_non_incr_thm >> gvs []
 QED
 
 Theorem eval_to'_def[compute,allow_rebind] =
@@ -682,320 +331,34 @@ Theorem eval_to'_def[compute,allow_rebind] =
 Theorem eval_to'_ind[allow_rebind] =
   REWRITE_RULE [fix_state_thm] eval_to'_ind;
 
-Theorem eval_to'_def[compute,allow_rebind] =
-  REWRITE_RULE [result_map'_fix_one] eval_to'_def;
-
-Theorem eval_to'_ind[allow_rebind] =
-  REWRITE_RULE [result_map'_fix_one] eval_to'_ind;
-
-Theorem eval_to'_def[compute,allow_rebind] =
-  REWRITE_RULE [result_map'_fix_two] eval_to'_def;
-
-Theorem eval_to'_ind[allow_rebind] =
-  REWRITE_RULE [result_map'_fix_two] eval_to'_ind;
-
-Definition eval'_def:
-  eval' x =
-    case some (c, t). FST (eval_to' <|c := c; t := t|> x) ≠ OOT of
-      NONE => Fail
-    | SOME (c, t) => FST (eval_to' <|c := c; t := t|> x)
-End
-
-Theorem eval_to'_add_lemma:
-  ∀s e v s' c t.
-    eval_to' s e = (Ok v, s')
-    ⇒ eval_to' <|c := s.c + c; t := s.t + t|> e
-        = (Ok v, <|c := s'.c + c; t := s'.t + t|>)
+Theorem eval_to'_add_thm:
+  (∀s e res s' sp.
+    eval_to' s e = (Ok res, s')
+    ⇒ eval_to' (s + sp) e = (Ok res, s' + sp)) ∧
+  (∀s xs rs s' sp.
+    result_map' s xs = (rs, s')
+    ∧ EVERY (isok ∘ FST) rs
+    ⇒ result_map' (s + sp) xs = (MAP (with_snd (λs. s + sp)) rs, s' + sp))
 Proof
   ho_match_mp_tac eval_to'_ind
-  >> rw []
-  >> gvs [AllCaseEqs(), eval_to'_def, check_state_def, fuel_def, trace_def]
-  >>~- ([`result_map' _ _ _ = _`],
-        imp_res_tac result_map'_add_thm
-        >> gvs []
-        >> first_x_assum $ qspec_then `<|c := c; t := t|>` assume_tac
-        >> gvs [])
-  >> qmatch_asmsub_abbrev_tac `<|c := a; t := b|>`
-  >> rpt (first_x_assum $ qspec_then `<|c := a; t := b|>` assume_tac
+  >> rw [eval_to'_def, check_state_def, fuel_def, trace_def]
+  >> gvs [AllCaseEqs()]
+  >>~- ([`mapok _ _`],
+        Cases_on `result_map' (state (s.c - 1) s.t) xs`
+        >> first_x_assum $ qspec_then `state (s.c - 1) s.t` assume_tac
+        >> gvs [AllCaseEqs()]
+        >> imp_res_tac mapok_every_thm >> gvs []
+        >> imp_res_tac mapok_add_thm
+        >> gvs [EVERY_MAP_WITH_FST_thm, EVERY_atom_lit_thm,
+                MAP_WITH_FST_WITH_SND_thm])
+  >>~- ([`result_map' _ _`],
+        Cases_on `eval_to' s e` >> gvs []
+        >> Cases_on `result_map' r xs` >> gvs []
+        >> Cases_on `q` >> gvs [with_snd_def])
+  >> qmatch_asmsub_abbrev_tac `state a b`
+  >> rpt (first_x_assum $ qspec_then `state a b` assume_tac
           >> gvs [])
   >> unabbrev_all_tac >> gvs []
 QED
 
-Theorem eval_to'_add_thm:
-  ∀s c t.
-    ∀e v s'.
-      eval_to' s e = (Ok v, s')
-      ⇒ eval_to' <|c := s.c + c; t := s.t + t|> e
-          = (Ok v, <|c := s'.c + c; t := s'.t + t|>)
-Proof
-  rw [eval_to'_add_lemma]
-QED
-
-Theorem eval_requiv_lemma:
-  ∀s e v s'. eval_to' s e = (Ok v, s')
-    ⇒ ∃c. eval_to c e = INR v
-Proof
-  cheat
-  (*ho_match_mp_tac eval_to'_ind
-  >> rw []
-  >> gvs [AllCaseEqs(), eval_to'_def, eval_to_def, check_state_def, fuel_def, trace_def]
-  >- (rpt (first_x_assum $ qspec_then `<|c := s.c - 1; t := s.t - 1|>` assume_tac
-           >> gvs [])
-      >> qexists `c + c' + c'' + 1`
-      >> qspecl_then [`c`, `c' + c'' + 1`] assume_tac eval_to_add_thm
-      >> pop_assum drule >> rw []
-      >> qspecl_then [`c'`, `c + c'' + 1`] assume_tac eval_to_add_thm
-      >> pop_assum drule >> rw []
-      >> Cases_on `fv` >> gvs [AllCaseEqs(), dest_anyClosure_def, dest_anyClosure'_def]
-      >> qspecl_then [`c''`, `c + c'`] assume_tac eval_to_add_thm
-      >> pop_assum drule >> rw [])
-  >- (first_x_assum $ qspec_then `<|c := s.c - 1; t := s.t|>` assume_tac
-      >> gvs []
-      >> qexists `c + 1` >> rw [])
-  >- (rpt (first_x_assum $ qspec_then `<|c := s.c - 1; t := s.t|>` assume_tac
-           >> gvs [])
-      >> qexists `c + c' + 1` >> rw []
-      >> qspecl_then [`c`, `c'`] assume_tac eval_to_add_thm
-      >> pop_assum drule >> rw []
-      >> qspecl_then [`c'`, `c`] assume_tac eval_to_add_thm
-      >> pop_assum drule >> rw [])
-  >- (rpt (first_x_assum $ qspec_then `<|c := s.c - 1; t := s.t|>` assume_tac
-           >> gvs [])
-      >> qexists `c + c' + 1` >> rw []
-      >> qspecl_then [`c`, `c'`] assume_tac eval_to_add_thm
-      >> pop_assum drule >> rw []
-      >> qspecl_then [`c'`, `c`] assume_tac eval_to_add_thm
-      >> pop_assum drule >> rw [])
-  >- (rpt (first_x_assum $ qspec_then `<|c := s.c - 1; t := s.t|>` assume_tac
-           >> gvs [])
-      >> qexists `c + c' + 1` >> rw []
-      >> qspecl_then [`c`, `c'`] assume_tac eval_to_add_thm
-      >> pop_assum drule >> rw []
-      >> qspecl_then [`c'`, `c`] assume_tac eval_to_add_thm
-      >> pop_assum drule >> rw [])
-  >- (rpt (first_x_assum $ qspec_then `<|c := s.c - 1; t := s.t|>` assume_tac
-           >> gvs [])
-      >> qexists `c + c' + 1` >> rw []
-      >> qspecl_then [`c`, `c'`] assume_tac eval_to_add_thm
-      >> pop_assum drule >> rw []
-      >> qspecl_then [`c'`, `c`] assume_tac eval_to_add_thm
-      >> pop_assum drule >> rw [])
-  >- (rpt (first_x_assum $ qspec_then `<|c := s.c - 1; t := s.t|>` assume_tac
-           >> gvs [])
-      >> qexists `c + c' + 1` >> rw []
-      >> qspecl_then [`c`, `c' + 1`] assume_tac eval_to_add_thm
-      >> pop_assum drule >> rw []
-      >> Cases_on `xv` >> gvs [AllCaseEqs(), dest_anyThunk_def, dest_anyThunk'_def]
-      >> qspecl_then [`c'`, `c`] assume_tac eval_to_add_thm
-      >> pop_assum drule >> rw [])*)
-QED
-
-Theorem really[simp]:
-  ∀s. <|c := s.c; t := s.t|> = s
-Proof
-  rw [fetch "-" "state_component_equality"]
-QED
-
-Theorem eval_lequiv_lemma:
-  ∀c e v.
-    eval_to c e = INR v
-    ⇒ ∃s s'. eval_to' s e = (Ok v, s')
-Proof
-  cheat
-  (*ho_match_mp_tac eval_to_ind
-  >> rw []
-  >> gvs [AllCaseEqs(), eval_to_def]
-  >> rw [AllCaseEqs(), eval_to'_def, check_state_def, fuel_def, trace_def]
-
-  >- (Cases_on `eval_to c e'` >> gvs []
-      >> Cases_on `eval_to c e` >> gvs []
-      >> Cases_on `y'` >> gvs [AllCaseEqs(), dest_anyClosure_def]
-      >- (first_x_assum $ qspecl_then [`[]`, `s'4'`, `y`, `e''`] assume_tac
-          >> gvs []
-          >> qexistsl [`<|c := s.c + s''.c + s'5'.c + 1; t := s.t + s''.t +
-                        s'5'.t + 1|>`, `<|c := s'.c + s'3'.c + s'6'.c; t :=
-                        s'.t + s'3'.t + s'6'.t|>`] >> gvs []
-          >> qspecl_then [`s''`, `s.c + s'5'.c`, `s.t + s'5'.t`] assume_tac eval_to'_add_thm
-          >> pop_assum drule >> rw []
-          >> rw [dest_anyClosure'_def]
-          >> qspecl_then [`s`, `s'3'.c + s'5'.c`, `s'3'.t + s'5'.t`] assume_tac
-               eval_to'_add_thm
-          >> pop_assum drule >> rw []
-          >> qspecl_then [`s'5'`, `s'.c + s'3'.c`, `s'.t + s'3'.t`] assume_tac
-               eval_to'_add_thm
-          >> pop_assum drule >> rw [])
-      >- (Cases_on `ALOOKUP (REVERSE l) s'4'` >> gvs []
-          >> Cases_on `x` >> gvs []
-          >> first_x_assum $ qspecl_then [`MAP (λ(g,x). (g,Recclosure l g)) l`,
-            `s'5'`, `y`, `e''`] assume_tac
-          >> gvs []
-          >> Cases_on `c = 0` >> gvs []
-          >> qexistsl [`<|c := s.c + s''.c + s'6'.c + 1; t := s.t + s''.t + s'6'.t + 1|>`,
-                       `<|c := s'.c + s'3'.c + s'7'.c; t := s'.t + s'3'.t + s'7'.t|>`]
-          >> gvs []
-          >> qspecl_then [`s''`, `s.c + s'6'.c`, `s.t + s'6'.t`] assume_tac eval_to'_add_thm
-          >> pop_assum drule >> rw []
-          >> rw [dest_anyClosure'_def]
-          >> qspecl_then [`s`, `s'3'.c + s'6'.c`, `s'3'.t + s'6'.t`] assume_tac eval_to'_add_thm
-          >> pop_assum drule >> rw []
-          >> qspecl_then [`s'6'`, `s'.c + s'3'.c`, `s'.t + s'3'.t`] assume_tac eval_to'_add_thm
-          >> pop_assum drule >> rw []))
-
-  >- (qexists `<|c := 1; t := 1|>` >> rw [])
-
-  >- (qexists `<|c := s.c + 1; t := s.t|>` >> rw [])
-
-  >- (Cases_on `eval_to (c - 1) e` >> gvs []
-      >> qexists `<|c := s.c + s''.c + 1; t := s.t + s''.t|>`
-      >> rw []
-      >> qspecl_then [`s`, `s''.c`, `s''.t`] assume_tac eval_to'_add_thm
-      >> pop_assum drule >> rw []
-      >> qspecl_then [`s''`, `s'.c`, `s'.t`] assume_tac eval_to'_add_thm
-      >> pop_assum drule >> rw [])
-  
-  >- (Cases_on `eval_to (c - 1) e` >> gvs []
-      >> first_x_assum $ drule_then assume_tac
-      >> gvs []
-      >> qexists `<|c := s.c + s''.c + 1; t := s.t + s''.t|>`
-      >> rw []
-      >> qspecl_then [`s`, `s''.c`, `s''.t`] assume_tac eval_to'_add_thm
-      >> pop_assum drule >> rw []
-      >> qspecl_then [`s''`, `s'.c`, `s'.t`] assume_tac eval_to'_add_thm
-      >> pop_assum drule >> rw [])
-
-  >- (Cases_on `eval_to (c - 1) e` >> gvs []
-      >> Cases_on `y` >> gvs []
-      >> Cases_on `b` >> gvs []
-      >> qexists `<|c := s.c + s''.c + 1; t := s.t + s''.t|>`
-      >> rw []
-      >> qspecl_then [`s`, `s''.c`, `s''.t`] assume_tac eval_to'_add_thm
-      >> pop_assum drule >> rw []
-      >> qspecl_then [`s''`, `s'.c`, `s'.t`] assume_tac eval_to'_add_thm
-      >> pop_assum drule >> rw [])
-
-  >- (qexists `<|c := 1; t := 1|>` >> rw [])
-
-  >- (Cases_on `eval_to c e` >> gvs [dest_anyThunk_def]
-      >> Cases_on `y` >> gvs []
-      >- (first_x_assum $ qspecl_then [`[]`, `e'`, `v`] assume_tac
-          >> gvs []
-          >> qexists `<|c := s.c + s''.c + 1; t := s.t + s''.t|>`
-          >> rw []
-          >> qspecl_then [`s`, `s''.c`, `s''.t`] assume_tac eval_to'_add_thm
-          >> pop_assum drule >> rw []
-          >> rw [dest_anyThunk'_def]
-          >> qspecl_then [`s''`, `s'.c`, `s'.t`] assume_tac eval_to'_add_thm
-          >> pop_assum drule >> rw [])
-      >- (Cases_on `ALOOKUP (REVERSE l) s''` >> gvs []
-          >> Cases_on `x` >> gvs []
-          >> first_x_assum $ qspecl_then [`l`, `e'`, `v`] assume_tac
-          >> gvs []
-          >> qexists `<|c := s.c + s'3'.c + 1; t := s.t + s'3'.t|>`
-          >> rw []
-          >> qspecl_then [`s`, `s'3'.c`, `s'3'.t`] assume_tac eval_to'_add_thm
-          >> pop_assum drule >> rw []
-          >> rw [dest_anyThunk'_def]
-          >> qspecl_then [`s'3'`, `s'.c`, `s'.t`] assume_tac eval_to'_add_thm
-          >> pop_assum drule >> rw []))
-
-  >- (qexists `<|c := 1; t := 1|>` >> rw [])*)
-QED
-
-Theorem eval_equiv_thm:
-  ∀e v.
-    (∀c. eval_to c e = INR v ⇒ ∃s s'. eval_to' s e = (Ok v, s')) ∧
-    (∀s s'. eval_to' s e = (Ok v, s') ⇒ ∃c. eval_to c e = INR v)
-Proof
-  rw []
-  >- (imp_res_tac eval_lequiv_lemma
-      >> metis_tac [])
-  >- (imp_res_tac eval_requiv_lemma
-      >> metis_tac [])
-QED
-
-Type inv = ``:state -> state -> bool``;
-
-Definition rel_def:
-  (val_rel (s : state) (q : inv) (Constructor n vs) (Constructor n' vs') ⇔
-    n = n' ∧ LIST_REL (val_rel s q) vs vs') ∧
-  (val_rel s q (Monadic op es) (Monadic op' es') ⇔
-    op = op' ∧ LIST_REL (exp_rel s (q, q)) es es') ∧
-  (val_rel s q (Closure x e) (Closure x' e') ⇔
-    ∀s' v1 v2.
-      if s'.c < s.c then
-        val_rel s' q v1 v2
-        ⇒ exp_rel s' (q, q) (subst1 x v1 e) (subst1 x' v2 e')
-      else
-        T) ∧
-  (val_rel s q (Recclosure fs n) (Recclosure fs' n') ⇔
-    ∀s' e e'.
-      s'.c < s.c
-      ∧ ALOOKUP fs n = SOME e
-      ∧ ALOOKUP fs' n' = SOME e'
-      ⇒
-      exp_rel s (q, q) (subst_funs fs e) (subst_funs fs' e')) ∧
-  (val_rel s q (Thunk e) (Thunk e') ⇔
-    exp_rel s (q, q) e e') ∧
-  (val_rel s q (Atom l) (Atom l') ⇔
-    l = l') ∧
-  (val_rel s q (DoTick v) (DoTick v') ⇔
-    val_rel s q v v') ∧
-  (val_rel s q v1 v2 ⇔ F) ∧
-
-  (res_rel (s : state) (q : inv) OOT OOT ⇔ T) ∧
-  (res_rel s q Fail Fail ⇔ T) ∧
-  (res_rel s q (Ok v) (Ok v') ⇔
-    val_rel s q v v') ∧
-  (res_rel s q r1 r2 ⇔ F) ∧
-
-  (exp_rel (s : state) ((ql, qg) : inv # inv) (e1 : exp) (e2 : exp) ⇔
-    ∀r1 s'.
-      s'.c ≤ s.c
-      ⇒ FST (eval_to' s' e1) = r1
-      ⇒ (∃r2 s''.
-          FST (eval_to' s'' e2) = r2 ∧
-          ql s' s'' ∧
-          res_rel <|c := s.c - s'.c; t := s.t|> qg r1 r2))
-Termination
-  cheat
-  (*WF_REL_TAC `inv_image ($< LEX ($< LEX $<))
-              (λx. case x of
-                   | INL (s, q, v1, v2) => (s.c, (v_size v1, 0))
-                   | INR (INL (s, q, r1, r2)) => (s.c, (res_size v_size r1, 1))
-                   | INR (INR (s, (ql,qg), e1, e2)) => (s.c, (exp_size e1, 2)))`
-  >- cheat*)
-End
-
-Definition subst_rel_def:
-  (subst_rel (s : state) (q : inv) (S : string set) (sub1 : (string # v) list) (sub2 : (string # v) list) ⇔  
-    ∀x v1.
-      if x ∈ S then
-        ALOOKUP sub1 x = SOME v1
-        ⇒ (∃v2. 
-            ALOOKUP sub2 x = SOME v2
-            ∧ val_rel s q v1 v2)
-      else
-        T)
-End
-
-Definition top_rel_def:
-  top_rel ((ql, qg) : inv # inv) (e1 : exp) (e2 : exp) ⇔
-    ∀(s : state) (sub1 : (string # v) list) (sub2 : (string # v) list).
-      subst_rel s qg (freevars e1) sub1 sub2
-      ⇒ (freevars e1) ⊆ (set (MAP FST sub1))
-      ⇒ exp_rel s (ql, qg) e1 e2
-End
-
-Definition constr_compat_thm:
-    ql <|c := 0; t := 0|> <|c := 0; t := 0|>
-    ∧ (∀c1 t1 c2 t2. ql <|c := c1; t := t1|> <|c := c2; t := t2|>
-                     ⇒ ql <|c := c1 + 1; t := t1|> <|c := c2 + 1; t := t2|>)
-    ⇒ ((∀vs1 vs2. LIST_REL (val_rel st qg) vs1 vs2
-        ⇒ exp_rel st (ql, qg) (subst1 x1 (Constructor n1 vs1) e1)
-                              (subst1 x2 (Constructor n2 vs2) e2))
-       ⇒ exp_rel st (ql, qg) (Let (SOME x1) (Value $ Constructor n1 es1) e1)
-                             (Let (SOME x2) (Value $ Constructor n2 es2) e2))
-Proof
-  cheat
-QED
-
+val _ = export_theory()
